@prefix cc: <http://creativecommons.org/ns#> .
@prefix dc: <http://purl.org/dc/terms/> .
@prefix li: <https://licensedb.org/ns#> .
@prefix owl: <http://www.w3.org/2002/07/owl#> .
@prefix rdf: <http://www.w3.org/1999/02/22-rdf-syntax-ns#> .
@prefix rdfs: <http://www.w3.org/2000/01/rdf-schema#> .
@prefix spdx: <http://spdx.org/rdf/terms#> .
@prefix xhv: <http://www.w3.org/1999/xhtml/vocab#> .
@prefix xsd: <http://www.w3.org/2001/XMLSchema-datatypes#> .
@prefix vann: <http://purl.org/vocab/vann/> .
@prefix wdrs: <http://www.w3.org/2007/05/powder-s#> .

<https://licensedb.org/ns#> rdf:type owl:Ontology ;
   dc:title """The License Database vocabulary"""@en-US ;
   dc:creator "Kuno Woudt <kuno@frob.nl>" ;
   dc:modified "2015-02-22" ;
   xhv:license <http://www.apache.org/licenses/LICENSE-2.0.html> ;
   vann:preferredNamespacePrefix "li" ;
   vann:preferredNamespaceUri "https://licensedb.org/ns#" ;
   rdfs:comment """## Introduction

There are a few situations where it would be useful to have a
machine-readable database of commonly used free culture and free
software licenses. The initial goal is to make this data available for
authoring and publishing software, to make it easier for creators to
pick any license they want and have the appropriate notices
automatically included when a copyrighted work is packaged for
distribution or published on a published platform.

The License Database vocabulary extends The Creative Commons Rights
Expression Language ([CC REL](http://wiki.creativecommons.org/CC_REL))
with additional properties to describe existing copyright and database
licenses in more detail.

[The License Database](https://licensedb.org/) project uses this
vocabulary to describe existing free software licenses, open source
licenses and free culture licenses used today.


## Status of this document

This is an editor's draft without any formal standing. It is not
endorsed by any organisation. Anything in this document is subject to
change, the editors welcome feedback on this document. Please send any
comments to [kuno@frob.nl](mailto:kuno@frob.nl) or contact "kuno" on
freenode irc.

"""@en-US .

li:License a rdfs:Class ;
   rdfs:comment """A standard text which can be applied by authors of
a creative work to license that work to users.  The standard text can
be copyright license, database rights license, trademark license,
patent grant, etc.."""@en-US ;
   rdfs:subClassOf cc:License, _:mustHaveTitle, _:mayHaveCreator,
      _:mayHaveIdentifier, _:mayHaveVersion .

_:mustHaveTitle a owl:Restriction ;
   owl:minCardinality 1 ;
   owl:onProperty dc:title .

_:mayHaveCreator a owl:Restriction ;
   owl:minCardinality 0 ;
   owl:onProperty dc:creator .

_:mayHaveIdentifier a owl:Restriction ;
   owl:minCardinality 0 ;
   owl:onProperty dc:identifier .

_:mayHaveVersion a owl:Restriction ;
   owl:minCardinality 0 ;
   owl:maxCardinality 1 ;
   owl:onProperty dc:hasVersion .


li:Notice a rdfs:Class ;
    rdfs:comment """A set of notices used to apply a particular license
to a work. Typically these notices disclaim warranty and state where
the full license text can be found. (If the license text is very short
this may contain the full license text).

Often the recommended (canonical) notices to use with a particular
license are a template where an author is expected to fill in their
details when using it to apply the license to a work -- this is
implemented in the License Database using the
[Mustache](http://mustache.github.com/mustache.5.html) template
language. The keys which may be used by a license notice template are:
{{year}}, {{rightsholder}}, {{description}} and {{title}}. """@en-US .


li:id a rdf:Property ;
   rdfs:domain li:License ;
   rdfs:range xsd:string ;
   rdfs:comment """The identifier assigned to the license by
the LicenseDB project. (the intent is to follow the same naming
scheme as defined in
[DEP5](http://dep.debian.net/deps/dep5/#license-specification))"""@en-US .

li:name a rdf:Property ;
   rdfs:domain li:License ;
   rdfs:range rdfs:Literal ;
   rdfs:comment """A short name assigned to the license. This should
be a short name suitable for display in a dropdown menu of a simple
license chooser or the copyright notice where there is limited room
for such notices.

For example, "CC BY-SA 3.0 NL" is the li:name for a creative commons
license which has "Attribution-ShareAlike 3.0 Netherlands" as
dc:title."""@en-US .

li:plaintext a rdf:Property ;
   rdfs:comment """The license is available as a plain text formatted
document at the linked resource.  This is usually the preferred format
to include in a packaged software project."""@en-US ;
   rdfs:domain li:License ;
   rdfs:range rdfs:Resource ;
   rdfs:subPropertyOf dc:hasFormat .

li:libre a rdf:Property ;
   rdfs:domain li:License ;
   rdfs:range rdfs:Resource ;
   rdfs:comment """This property states that a license is suitable for
use in free software, open source software, free culture or open data
according to a particular organization."""@en-US .

li:compatible a rdf:Property ;
   rdfs:domain li:License ;
   rdfs:range li:License ;
   rdfs:comment """This property states that works under these licenses
can be combined into a single work."""@en-US .


li:text a rdf:Property ;
   rdfs:comment "The text used to apply a license to a work."@en-US ;
   rdfs:domain li:License ;
   rdfs:range rdfs:Literal .

li:short a rdf:Property ;
   rdfs:comment """A boolean, if true signifies that this particular
notice is a short notice typically used in user interfaces where there
is not enough room for a longer text. If false the notice is a slightly
longer text typically used in software source code files and
[README](http://en.wikipedia.org/wiki/README) files or anywhere else
where there is sufficient room for a slightly longer text."""@en-US ;
   rdfs:domain li:Notice ;
   rdfs:range xsd:boolean .

li:orlater a rdf:Property ;
   rdfs:comment """A boolean, if true signifies that this particular
notice is a notice typically used to apply an "or-later" clause to a
versioned license. If false the notice will not allow the licensee to
upgrade to a newer version of the license."""@en-US ;
   rdfs:domain li:Notice ;
   rdfs:range xsd:boolean .

li:canonical a rdf:Property ;
   rdfs:comment """A boolean, if true signifies that this particular
notice is a canonical notice recommended by the publisher of the license
(e.g. in the license text itself). This is also set as "true" for short
(permissive) licenses where the notice is the full license."""@en-US ;
   rdfs:domain li:Notice ;
   rdfs:range xsd:boolean .
